adding back inductive pred

Arith/Instrs.lean
@@ -1,41 +1,72 @@
+import «Arith».Types
+
 abbrev Reg := Nat
+-- def Reg := Nat
+
+-- instance : OfNat Reg 0 where
+--   ofNat := Nat.zero
+
+-- instance : OfNat Reg n where
+--   ofNat := n
+
+-- instance : Repr Reg where
+--   reprPrec : Reg -> Nat -> Std.Format
+--   | 0, _ => "rax"
+--   | r, _ => "r" ++ (Nat.repr r)
+
+-- instance : ToString Reg where
+--   toString : Reg -> String
+--   | 0 => "rax"
+--   | r => "r" ++ (Nat.repr r)
+
+instance : BEq Reg where
+  beq := Nat.beq
+
+instance : Add Reg where
+  add := Nat.add
+
 abbrev Accum := Nat
 abbrev Flag := Nat
 abbrev Mem := Reg -> Nat
 abbrev ProgCnt := Nat
 abbrev Config := Accum × Flag × ProgCnt × Mem
 
-def empty : Mem := fun _ => 0
+@[simp] def empty : Mem := fun x => 0
 
-def get (r : Reg) (m : Mem) : Nat := m r
+@[simp] def get (r : Reg) (m : Mem) : Nat := m r
 
-def set (r : Reg) (n : Nat) (m : Mem) : Mem := fun r' => if r == r' then n else get r' m
+@[simp] def set (r : Reg) (n : Nat) (m : Mem) : Mem := fun r' => if r == r' then n else get r' m
 
-def first : Reg := 1
+@[simp] def first : Reg := 1
 
-def next (r : Reg) : Reg := r + 1
+@[simp] def next (r : Reg) : Reg := r + 1
 
-def rax : Reg := 0
+@[simp] def rax : Reg := 0
 
 inductive Instr : Type
-| mov   : Reg -> Reg -> Instr
-| movi  : Reg -> Nat -> Instr
-| add   : Reg -> Reg -> Instr
-| addi  : Reg -> Nat -> Instr
-| sub   : Reg -> Reg -> Instr
-| subi  : Reg -> Nat -> Instr
-| xor   : Reg -> Nat -> Instr
-| and   : Reg -> Nat -> Instr
-| sar   : Reg -> Nat -> Instr
-| sal   : Reg -> Nat -> Instr
-| cmp   : Reg -> Reg -> Instr
-| cmpi  : Reg -> Nat -> Instr
-| jmp   : Nat -> Instr
-| je    : Nat -> Instr
-| jne   : Nat -> Instr
-| jl    : Nat -> Instr
-| jg    : Nat -> Instr
-deriving Repr
+| mov      : Reg -> Reg -> Instr
+| movi     : Reg -> Nat -> Instr
+| add      : Reg -> Reg -> Instr
+| addi     : Reg -> Nat -> Instr
+| sub      : Reg -> Reg -> Instr
+| subi     : Reg -> Nat -> Instr
+| xor      : Reg -> Nat -> Instr
+| and      : Reg -> Nat -> Instr
+| sar      : Reg -> Nat -> Instr
+| sal      : Reg -> Nat -> Instr
+| cmp      : Reg -> Reg -> Instr
+| cmpi     : Reg -> Nat -> Instr
+| jmp      : Nat -> Instr
+| je       : Nat -> Instr
+| jne      : Nat -> Instr
+| jl       : Nat -> Instr
+| jg       : Nat -> Instr
+| halt     : Instr
+| halteq   : Instr
+| haltne   : Instr
+| haltg    : Instr
+| haltl    : Instr
+deriving Repr, BEq
 
 inductive SmallStep : Instr -> Config -> Config -> Prop
 | mov {acc flag i mem} (r1 : Reg) (r2 : Reg):
@@ -128,3 +159,65 @@ inductive SmallStep : Instr -> Config -> Config -> Prop
   SmallStep (Instr.jl n) (acc, flag, i, mem) (acc, flag, i + n + 1, mem)
 | jg_false {acc flag i mem} (n : Nat) (fcond : flag != 2):
   SmallStep (Instr.jl n) (acc, flag, i, mem) (acc, flag, i + 1, mem)
+mutual
+  @[simp] def exec1 (prog : Prog) (c : Config) : Prog × Config :=
+    match c with
+    | (acc, flag, mem) => (match prog with
+      | [] => (prog, c)
+      | (mov r1 0)::ps      => exec1 ps (acc, flag, set r1 acc mem)
+      | (mov 0 r2)::ps      => exec1 ps (get r2 mem, flag, mem)
+      | (mov r1 r2)::ps     => exec1 ps (acc, flag, set r1 (get r2 mem) mem)
+      | (movi 0 imm)::ps    => exec1 ps (imm, flag, mem)
+      | (movi r1 imm)::ps   => exec1 ps (acc, flag, set r1 imm mem)
+      | (addi 0 imm)::ps    => exec1 ps (acc + imm, flag, mem)
+      | (addi r1 imm)::ps   => exec1 ps (acc, flag, set r1 ((get r1 mem) + imm) mem)
+      | (subi 0 imm)::ps    => exec1 ps (acc - imm, flag, mem)
+      | (subi r1 imm)::ps   => exec1 ps (acc, flag, set r1 ((get r1 mem) - imm) mem)
+      | (add 0 r2)::ps      => exec1 ps (acc + get r2 mem, flag, mem)
+      | (add r1 0)::ps      => exec1 ps (acc, flag, set r1 (get r1 mem + acc) mem)
+      | (add r1 r2)::ps     => exec1 ps (acc, flag, set r1 ((get r1 mem) + (get r2 mem)) mem)
+      | (sub 0 r2)::ps      => exec1 ps (acc - get r2 mem, flag, mem)
+      | (sub r1 0)::ps      => exec1 ps (acc, flag, set r1 (get r1 mem - acc) mem)
+      | (sub r1 r2)::ps     => exec1 ps (acc, flag, set r1 ((get r1 mem) - (get r2 mem)) mem)
+      | (Instr.xor rax imm)::ps   => exec1 ps (acc ^^^ imm, flag, mem)
+      | (Instr.and 0 imm)::ps     => exec1 ps (acc &&& imm, flag, mem)
+      | (Instr.and r1 imm)::ps    => exec1 ps (acc, flag, set r1 (get r1 mem &&& imm) mem)
+      | (sar rax imm)::ps   => exec1 ps (acc >>> imm, flag, mem)
+      | (sal rax imm)::ps   => exec1 ps (acc <<< imm, flag, mem)
+      | (cmp 0 r2)::ps      =>
+          let v := get r2 mem
+          let flag' := if (acc == v) then 0 else (if acc < v then 1 else 2)
+          exec1 ps (acc, flag', mem)
+      | (cmp r1 r2)::ps     =>
+          let v1 := get r1 mem
+          let v2 := get r2 mem
+          let flag' := if (v1 == v2) then 0 else (if v1 < v2 then 1 else 2)
+          exec1 ps (acc, flag', mem)
+      | (cmpi 0 imm)::ps    =>
+          let flag' := if (acc == imm) then 0 else (if acc < imm then 1 else 2)
+          exec1 ps (acc, flag', mem)
+      | (cmpi r1 imm)::ps   =>
+          let v := get r1 mem
+          let flag' := if (v == imm) then 0 else (if v < imm then 1 else 2)
+          exec1 ps (acc, flag', mem)
+      | (jmp n)::ps         => jump_forward ps c n
+      | (je n)::ps          => if flag == 0 then jump_forward ps c n else exec1 ps (acc, flag, mem) -- other instructions
+      | (jne n)::ps         => if flag != 0 then jump_forward ps c n else exec1 ps (acc, flag, mem)
+      | (jl n)::ps          => if flag == 1 then jump_forward ps c n else exec1 ps (acc, flag, mem)
+      | (jg n)::ps          => if flag == 2 then jump_forward ps c n else exec1 ps (acc, flag, mem)
+      | halt::ps            => (ps, (acc, flag, mem))
+      | halteq::ps          => if flag == 0 then (ps, (acc, flag, mem)) else exec1 ps (acc, flag, mem)
+      | haltne::ps          => if flag != 0 then (ps, (acc, flag, mem)) else exec1 ps (acc, flag, mem)
+      | haltl::ps           => if flag == 1 then (ps, (acc, flag, mem)) else exec1 ps (acc, flag, mem)
+      | haltg::ps           => if flag == 2 then (ps, (acc, flag, mem)) else exec1 ps (acc, flag, mem))
+  @[simp] def jump_forward (prog : Prog) (c : Config) (n : Nat) : Prog × Config :=
+    match prog, n with
+    | [], _                 => ([], c)
+    | ps, 0                 => exec1 ps c
+    | _::ps, Nat.succ n'    => jump_forward ps c n'
+end
+
+@[simp] def exec (prog : Prog) : Nat :=
+  match exec1 prog (0, 0, empty) with
+  | ([], c) => c.fst
+  | (_, _)  => val_void
