Arith.lean
@@ -2,3 +2,8 @@
 -- Import modules here that should be built as part of the library.
 import «Arith».AST
 import «Arith».Example
+import «Arith».Instrs
+import «Arith».Types
+import «Arith».Compile
+import «Arith».Eval
+import «Arith».Proof
