Arith/Compile.lean
@@ -1,0 +1,120 @@
+import «Arith».Instrs
+import «Arith».AST
+import «Arith».Types
+open Instr
+open Convertible
+
+abbrev Context := List (ID × Reg)
+
+@[simp] def lookup (x : ID) (c : Context) : Except String Reg :=
+  match c with
+  | [] => throw s!"variable {x} not in context"
+  | (var, reg) :: cs => if var == x then (pure reg) else lookup x cs
+
+@[simp] def assertType (mask : Nat) (type : Nat) (r : Reg) : StateT Reg (Except String) Prog := do
+  let r' <- get
+  set (next r')
+  return [
+    mov r' r, 
+    and r' mask,
+    cmpi r' type,
+    haltne
+  ]
+
+@[simp] def typePred (mask : Nat) (type : Nat) : Prog :=
+  [and rax mask, cmpi rax type, mov rax (valToBits true), je 1, mov rax (valToBits false)]
+
+@[simp] def assertInteger := assertType int_mask type_int
+
+@[simp] def assertChar := assertType char_mask type_char
+
+@[simp] def assertCodepoint (r : Reg) : StateT Reg (Except String) Prog := do
+  let check <- assertInteger r
+  return (
+    check ++
+   [cmpi r (valToBits 0),
+    haltl, 
+    cmpi rax (valToBits 1114111),
+    haltg, 
+    cmpi rax (valToBits 55295),
+    jl 3,
+    cmpi rax (valToBits 57344),
+    jg 1,
+    halt 
+   ])
+
+@[simp] def compileVal (val : α) [Convertible α] : Prog := 
+  [movi rax (valToBits val)]
+
+@[simp] def compile_op1 (op : Op1) : StateT Reg (Except String) Prog :=
+  match op with
+  | .add1 => do
+      let check <- assertInteger rax
+      return (check ++ [addi rax (valToBits 1)])
+  | .sub1 => do
+      let check <- assertInteger rax
+      return (check ++ [subi rax (valToBits 1)])
+  -- | .zerohuh => do
+  --     let check <- assertInteger rax
+  --     return (
+  --       check ++ 
+  --      [cmpi rax 0,
+  --       movi rax val_true,
+  --       je 1,
+  --       movi rax val_false])
+  -- | .charhuh => return (typePred char_mask type_char)
+  -- | .chartoint => do
+  --     let check <- assertChar rax
+  --     return (
+  --       check ++
+  --      [sar rax char_shift,
+  --       sal rax int_shift])
+  -- | .inttochar => do
+  --     let check <- assertCodepoint rax
+  --     return (
+  --       check ++ 
+  --      [sar rax int_shift,
+  --       sal rax char_shift,
+  --       xor rax type_char])
+  -- | .neg => do
+  --     let check <- assertInteger rax
+  --     let r <- get
+  --     set (next r)
+  --     return 
+
+  | _ => return []
+
+mutual
+@[simp] def compile_expr (e : Expr) (c : Context) : StateT Reg (Except String) Prog :=
+  match e with
+  | .integer n    => return (compileVal n)
+  | .boolean b    => return (compileVal b)
+  | .character c  => return (compileVal c)
+  | .var x        => do
+      let reg <- lookup x c
+      return [mov rax reg]
+  | .prim1 op e => do
+      let instrs <- compile_expr e c
+      let instrs' <- compile_op1 op
+      return (instrs ++ instrs')
+  | .letstd ids es body => do
+      let (regs, progs) <- compile_star es c
+      let prog <- compile_expr body ((List.zip ids regs) ++ c)
+      return (progs ++ prog)
+  | _ => return [mov rax 1]
+
+@[simp] def compile_star (es : List Expr) (c : Context) : StateT Reg (Except String) ((List Reg) × Prog) :=
+  match es with
+  | []    => return ([], [])
+  | e::es => do
+      let e_instrs <- compile_expr e c
+      let r <- get
+      set (next r)
+      let (rs, es_instrs) <- compile_star es c
+      return (r::rs, e_instrs ++ [mov r rax] ++ es_instrs)
+end
+
+@[simp] def compile (e : Expr) : Except String Prog :=
+  match (compile_expr e [] first) with
+  | .ok res => return res.fst
+  | .error _ => throw "compile err"
