Arith/Eval.lean
@@ -1,0 +1,61 @@
+import «Arith».AST
+import «Arith».Types
+open Convertible
+
+inductive Value where
+| num (n : Nat)
+| bool (b : Bool)
+| char (c : Char)
+
+abbrev Env := List (ID × Value)
+
+@[simp] def lookup_env (r : Env) (x : ID) : Except String Value :=
+  match r with 
+  | [] => throw s!"variable {x} not found in environment"
+  | (id, v)::rs => if id == x then (return v) else lookup_env rs x
+
+open Value
+
+@[simp] def interpPrim1 (op : Op1) (e : Value) : Except String Value :=
+  match op with 
+  | .add1 => 
+      (match e with 
+      | .num n => return (.num (n + 1))
+      | _ => throw s!"add1 requires nat argument")
+  | .sub1 => 
+    (match e with 
+      | .num n => return (.num (n - 1))
+      | _ => throw s!"sub1 requires nat argument")
+  | _ => return (.num 1)
+
+mutual
+@[simp] def interp_env (e : Expr) (r : Env) : Except String Value :=
+  match e with
+  | .integer n => return (num n)
+  | .boolean b => return (bool b)
+  | .character c => return (char c)
+  | .var x => lookup_env r x
+  | .prim1 op e => do
+      let v <- interp_env e r
+      interpPrim1 op v
+  | .letstd ids es body => do
+      let vs <- interp_star es r
+      interp_env body ((List.zip ids vs) ++ r)
+  | _ => return (num 1)
+
+@[simp] def interp_star (es : List Expr) (r : Env) : Except String (List Value) :=
+  match es with
+  | []    => return []
+  | e::es => do
+    let v <- interp_env e r
+    let vs <- interp_star es r
+    return (v::vs)
+end
+
+@[simp] def interp (e : Expr) : Nat :=
+  match interp_env e [] with
+  | .error _ => val_void
+  | .ok res => (match res with 
+    | .num n => valToBits n
+    | .bool b => valToBits b
+    | .char c => valToBits c)
