Arith/Example.lean
@@ -1,1 +1,9 @@
 import «Arith».AST
+
+open Expr
+open OpN
+--open Op0
+open Op1
+open Op2
+
+def exampl : Expr := letstd ["x","y"] [integer 1,integer 2] (var "x")
