Arith/Proof.lean
@@ -1,0 +1,34 @@
+import «Arith».Compile
+import «Arith».Eval
+import «Arith».Instrs
+import «Arith».AST
+import Aesop
+
+open Op1
+
+theorem concat_prog:
+  ∀ (e : Expr) (prog' : Prog) (config : Config),
+    match (compile e) with
+    | Except.ok prog => let (_, config') := exec1 prog config
+                        exec1 (prog ++ prog') config = exec1 prog' config'
+    | Except.error _ => true
+  | _ => by sorry
+
+theorem correctness:
+    ∀ (e : Expr),
+      match (compile e) with
+      | Except.ok prog => (exec prog = interp e)
+                          --let (prog', (res, _, _)) := exec1 prog (0, 0, empty)
+                          --((prog' == []) -> res == interp e) || ((prog' != []) -> interp e == val_void)
+      | Except.error _   => interp e = val_void
+  | .integer n => by simp [pure, Except.pure, StateT.pure, Convertible.valToBits]
+  | .boolean b => by simp [pure, Except.pure, StateT.pure, Convertible.valToBits]
+  | .character c => by simp [pure, Except.pure, StateT.pure, Convertible.valToBits]
+  | .var x => by simp [Except.pure, StateT.pure,
+                      bind, Except.bind, StateT.bind,
+                      liftM, monadLift, MonadLift.monadLift, StateT.lift,
+                      Convertible.valToBits]
+  | .prim1 (Op1.add1) e => by
+    have ih := correctness e
+    simp
+  | _ => by sorry
